Complete stack machine and compilation of arith.

ASM.thy
@@ -4,38 +4,40 @@ theory ASM imports AExp begin
 
 subsection "Stack Machine"
 
-(* The stack machine has three instructions: *)
-datatype instr = LOADI val
-               | LOAD vname
-               | ADD
+(* The stack machine instructions. *)
+datatype instr =
+  LOADI val
+| LOAD vname
+| ADD
+| TIMES
 
-(* The semantics:
-   + LOADI n puts the immediate n on top of the stack,
-   + LOAD x puts the value of x on top of the stack, and
-   + ADD replaces the two topmost elements by their sum. *)
+(* The semantics is
+   + LOADI n puts the immediate n on top of the sta\<^bold>ck;
+   + LOAD x puts the value of x on top of the stack;
+   + ADD replaces the first two elements by their sum. *)
 
-(* A stack: *)
 type_synonym stack = "val list"
-(* The top of the stack is the head of the list *)
+(* The top of the stack is the head of the list. *)
 
-(* An instruction is executed in the context of a state and transforms a stack into a new stack. *)
+(* An instruction is executed in the context of a state
+   and transforms a stack into a new stack. *)
 fun exec1 :: "instr \<Rightarrow> state \<Rightarrow> stack \<Rightarrow> stack" where
   "exec1 (LOADI n) _ stack = n # stack"
-| "exec1 (LOAD x) s stack = s x # stack"
+| "exec1 (LOAD x) s stack = (s x) # stack"
 | "exec1 ADD _ (j # i # stack) = (i + j) # stack"
+| "exec1 TIMES _ (j # i # stack) = (i * j) # stack"
 
 (* A list of instructions is executed one by one. *)
 fun exec :: "instr list \<Rightarrow> state \<Rightarrow> stack \<Rightarrow> stack" where
   "exec [] _ stack = stack"
-| "exec (i # is) s stack = exec is s (exec1 i s stack)"
+| "exec (i # rest) s stack = exec rest s (exec1 i s stack)"
 
-value "exec [LOADI 5, LOAD ''y'', ADD]
-      <''x'' := 42, ''y'' := 43> [50]"
+lemma "exec [LOADI 5, LOAD ''y'', ADD]
+      <''x'' := 42, ''y'' := 43> [50] = [48, 50]" by simp
 
-lemma exec_append [simp]: "exec (is1 @ is2) s stack = exec is2 s (exec is1 s stack)"
-apply (induction is1 arbitrary: stack)
-apply auto
-done
+lemma exec_append [simp]: "exec (is1 @ is2) s stack
+                           = exec is2 s (exec is1 s stack)"
+by (induct is1 arbitrary: stack, auto)
 
 subsection "Compilation"
 
@@ -44,14 +46,13 @@ fun comp :: "aexp \<Rightarrow> instr list" where
   "comp (N n) = [LOADI n]"
 | "comp (V x) = [LOAD x]"
 | "comp (Plus e1 e2) = comp e1 @ comp e2 @ [ADD]"
+| "comp (Times e1 e2) = comp e1 @ comp e2 @ [TIMES]"
 
 value "comp (Plus (Plus (V ''x'') (N 1)) (V ''z''))"
 
 (* The correctness statement says that executing a compiled expression
    is the same as putting the value of the expression on the stack: *)
 theorem exec_comp: "exec (comp a) s stack = aval a s # stack"
-apply (induction a arbitrary: stack)
-apply auto
-done
+by (induction a arbitrary: stack, auto)
 
 end
